doc/simple/coq/Exists.v
@@ -1,0 +1,582 @@
+Require Import CtxExtension.
+Require Import LibLN.
+Require Import AlgoDef.
+Require Import UtilityEnv.
+Require Import DeclDef.
+Require Import DeclInfra.
+Require Import AlgoInfra.
+Require Import Subst.
+Require Import LibReflect.
+
+Definition cpltctxsubst_exists_def := forall G e,
+    AWf G ->
+    AWTerm G e ->
+    CompleteCtx G ->
+    exists t, ACpltCtxSubst G e t
+.
+
+Definition cpltctxtsubst_exists_def := forall G e,
+    AWf G ->
+    AWTermT G e ->
+    CompleteCtx G ->
+    exists t, ACpltCtxTSubst G e t
+.
+
+(* admitted lemma with issue about quantification *)
+
+Lemma lam_solve: forall G x e t,
+    AWf (G & x ~ AC_Var) ->
+    ACpltCtxSubst (G & x ~ AC_Var) (e @ x) t ->
+    exists d, ACpltCtxSubst G (AE_Lam e) d.
+Admitted.
+
+Lemma pi_solve: forall G x e1 e2 t1 t2,
+    AWf (G & x ~ AC_Var) ->
+    ACpltCtxSubst G e1 t1 ->
+    ACpltCtxSubst (G & x ~ AC_Var) (e2 @ x) t2 ->
+    exists d, ACpltCtxSubst G (AE_Pi e1 e2) d.
+Admitted.
+
+Lemma let_solve: forall G x e1 e2 t1 t2,
+    AWf (G & x ~ AC_Var) ->
+    ACpltCtxSubst G e1 t1 ->
+    ACpltCtxSubst (G & x ~ AC_Var) (e2 @ x) t2 ->
+    exists d, ACpltCtxSubst G (AE_Let e1 e2) d.
+Admitted.
+
+Lemma forall_solve: forall G x e t,
+    AWf (G & x ~ AC_Var) ->
+    ACpltCtxTSubst (G & x ~ AC_Var) (e @' x) t ->
+    exists d, ACpltCtxTSubst G (AT_Forall e) d.
+Admitted.
+
+(* another form of awterm, which does not care about bound variables *)
+
+Inductive AWTermA : ACtx -> AExpr -> Prop :=
+  | AWTermA_Var : forall G x, binds x AC_Var G -> AWTermA G (AE_FVar x)
+  | AWTermA_BVar : forall G x, AWTermA G (AE_BVar x)
+  | AWTermA_TypVar : forall G x t, binds x (AC_Typ t) G -> AWTermA G (AE_FVar x)
+  | AWTermA_LetVar : forall G x t e, binds x (AC_Bnd t e) G -> AWTermA G (AE_FVar x)
+  | AWTermA_EVar : forall G a, binds a AC_Unsolved_EVar G -> AWTermA G (AE_EVar a)
+  | AWTermA_Solved_EVar : forall G a t, binds a (AC_Solved_EVar t) G -> AWTermA G (AE_EVar a)
+  | AWTermA_Star: forall G, AWTermA G AE_Star
+  | AWTermA_App: forall e1 e2 G, AWTermA G e1 -> AWTermA G e2 -> AWTermA G (AE_App e1 e2)
+  | AWTermA_Lam: forall e G , AWTermA G e  -> AWTermA G (AE_Lam e)
+  | AWTermA_Pi: forall t1 t2 G, AWTermA G t1 -> AWTermA G t2 -> AWTermA G (AE_Pi t1 t2)
+  | AWTermA_Let: forall e1 e2 G, AWTermA G e1 -> AWTermA G e2 -> AWTermA G (AE_Let e1 e2)
+  | AWTermA_CastUp : forall e G, AWTermA G e -> AWTermA G (AE_CastUp e)
+  | AWTermA_CastDn : forall e G, AWTermA G e -> AWTermA G (AE_CastDn e)
+  | AWTermA_Ann: forall e1 e2 G, AWTermA G e1 -> AWTermA G e2 -> AWTermA G (AE_Ann e1 e2)
+.
+
+(* helper lemmas *)
+Hint Constructors AWTermA ACpltCtxSubst.
+Lemma cpltctxsubst_solved_weaken: forall G1 G2 t e,
+    AWf (G1 & G2) ->
+    CompleteCtx (G1 & G2) ->
+    AWTerm G1 t ->
+    ACpltCtxSubst (G1 & G2) t e ->
+    ACpltCtxSubst G1 t e.
+Proof.
+  introv wf compl wt sub. gen_eq H:(G1& G2).
+  induction sub; introv HG.
+  inversion wt; subst.
+Admitted.
+  (* apply ACpltCtxSubst *)
+  (* induction t. *)
+  (* inversion sub; subst. *)
+  (* inversion sub; subst. *)
+  (* admit. *)
+(* Qed. *)
+
+Lemma awterma_open: forall G k u e,
+    AWTermA G (AOpenRec k u e) ->
+    AWTermA G e.
+Proof.
+  introv wt. gen k u. induction e; intros; simpls; auto_star;
+  try(inversion wt; subst; auto_star).
+Qed.
+
+Lemma awterma_remove: forall G H e y v,
+    AWTermA (G & y ~ v & H) e ->
+    y \notin AFv e ->
+    AWTermA (G & H) e.
+Proof.
+  introv wt notin. gen_eq I: (G & y ~ v & H).
+  gen H. induction wt; introv hh; auto_star.
+  simpl in notin. rewrite hh in H. apply AWTermA_Var. apply* binds_subst.
+  simpl in notin. rewrite hh in H. apply* AWTermA_TypVar. apply* binds_subst.
+  simpl in notin. rewrite hh in H. apply* AWTermA_LetVar. apply* binds_subst.
+  simpl in notin. rewrite hh in H. apply* AWTermA_EVar. apply* binds_subst.
+  simpl in notin. rewrite hh in H. apply* AWTermA_Solved_EVar. apply* binds_subst.
+
+  simpl in notin. apply AWTermA_App. apply* IHwt1. apply* IHwt2.
+
+  simpl in notin. apply AWTermA_Pi. apply* IHwt1. apply* IHwt2.
+  simpl in notin. apply AWTermA_Let. apply* IHwt1. apply* IHwt2.
+  simpl in notin. apply AWTermA_Ann. apply* IHwt1. apply* IHwt2.
+Qed.
+
+Lemma awterma_remove_empty: forall G e y v,
+    AWTermA (G & y ~ v) e ->
+    y \notin AFv e ->
+    AWTermA G e.
+Proof.
+  intros. assert (AWTermA (G & y ~ v & empty) e). rewrite* concat_empty_r.
+  assert (AWTermA (G & empty) e). apply* awterma_remove.
+  rewrite concat_empty_r in H2. auto.
+Qed.
+
+(* one important one, changes from awterm to awterma *)
+
+Theorem awterm_is_awterma: forall G e,
+    AWTerm G e ->
+    AWTermA G e.
+Proof.
+  introv wt. induction wt; auto_star.
+  pick_fresh y. assert (AWTermA (G & y ~ AC_Var) (e @ y)).
+  apply H0. auto_star. apply awterma_open in H1. apply awterma_remove_empty in H1. constructor*. auto_star.
+  constructor*. pick_fresh y. assert (AWTermA (G & y ~ AC_Var) (t2 @ y)).
+  apply H0. auto_star. apply awterma_open in H1. apply awterma_remove_empty in H1. auto_star. auto_star.
+  constructor*. pick_fresh y. assert (AWTermA (G & y ~ AC_Var) (e2 @ y)).
+  apply H0. auto_star. apply awterma_open in H1. apply awterma_remove_empty in H1. auto_star. auto_star.
+Qed.
+
+(* a definition about length of a expression.
+( in order to make all the expression has length,
+( there are many meaningless definition,
+( which ends with `I` *)
+
+Inductive ALen : ACtx -> AExpr -> nat -> Prop :=
+| ALen_BVar: forall G i, ALen G (AE_BVar i) 1
+| ALen_Var: forall G x, binds x AC_Var G -> ALen G (AE_FVar x) 1
+| ALen_TypVar: forall G x t, binds x (AC_Typ t) G -> ALen G (AE_FVar x) 1
+| ALen_LetVar : forall G x t e i, binds x (AC_Bnd t e) G -> ALen G e i -> ALen G (AE_FVar x) (i + 1)
+| ALen_Var_I1 : forall G x, binds x AC_Unsolved_EVar G -> ALen G (AE_FVar x) 1
+| ALen_Var_I2 : forall G x t, binds x (AC_Solved_EVar t) G -> ALen G (AE_FVar x) 1
+| ALen_Var_I : forall G x, x # G -> ALen G (AE_FVar x) 1
+| ALen_EVar : forall G a, binds a AC_Unsolved_EVar G -> ALen G (AE_EVar a) 1
+| ALen_EVar_I1: forall G x, binds x AC_Var G -> ALen G (AE_EVar x) 1
+| ALen_EVar_I2: forall G x t, binds x (AC_Typ t) G -> ALen G (AE_EVar x) 1
+| ALen_EVar_I3: forall G x t e, binds x (AC_Bnd t e) G -> ALen G (AE_EVar x) 1
+| ALen_Solved_EVar: forall G a t i, binds a (AC_Solved_EVar t) G -> ALen G t i -> ALen G (AE_EVar a) (i + 1)
+| ALen_EVar_I : forall G a, a # G -> ALen G (AE_EVar a) 1
+| ALen_Star: forall G, ALen G (AE_Star) 1
+| ALen_App: forall e1 e2 G i1 i2, ALen G e1 i1 -> ALen G e2 i2 -> ALen G (AE_App e1 e2) (i1 + i2 + 1)
+| ALen_Lam: forall e G i, ALen G e i -> ALen G (AE_Lam e) (i + 1)
+| ALen_Pi: forall e1 e2 G i1 i2, ALen G e1 i1 -> ALen G e2 i2 -> ALen G (AE_Pi e1 e2) (i1 + i2 + 1)
+| ALen_Let: forall e1 e2 G i1 i2, ALen G e1 i1 -> ALen G e2 i2 -> ALen G (AE_Let e1 e2) (i1 + i2 + 1)
+| ALen_CastUp:  forall e G i, ALen G e i -> ALen G (AE_CastUp e) (i + 1)
+| ALen_CastDn:  forall e G i, ALen G e i -> ALen G (AE_CastDn e) (i + 1)
+| ALen_Ann: forall e1 e2 G i1 i2, ALen G e1 i1 -> ALen G e2 i2 -> ALen G (AE_Ann e1 e2) (i1 + i2 + 1).
+
+Hint Constructors ALen.
+
+(* some lemmas about alen *)
+
+Lemma alen_add_var': forall G e i y m,
+    ALen G e i ->
+    i < m ->
+    ok (G & y ~ AC_Var) ->
+    ALen (G & y ~ AC_Var) e i.
+Proof.
+  introv. gen G e i y. induction m.
+  introv len less okg.
+  inversion less.
+
+  introv len less okg.
+  gen i. induction e; introv len less.
+  inversion len; subst. apply ALen_BVar.
+  inversion len; subst.
+  assert (v<>y). intros neq. subst. apply ok_push_inv in okg. destruct okg as [_ okg]. false binds_fresh_inv H1 okg.
+  apply ALen_Var. apply* binds_concat_left.
+
+  assert (v<>y). intros neq. subst. apply ok_push_inv in okg. destruct okg as [_ okg]. false binds_fresh_inv H1 okg.
+  apply ALen_TypVar with t. apply* binds_concat_left.
+
+  assert (v<>y). intros neq. subst. apply ok_push_inv in okg. destruct okg as [_ okg]. false binds_fresh_inv H0 okg.
+  apply ALen_LetVar with t e. apply* binds_concat_left.
+  apply* IHm. Omega.omega.
+
+  assert (v<>y). intros neq. subst. apply ok_push_inv in okg. destruct okg as [_ okg]. false binds_fresh_inv H1 okg.
+  apply ALen_Var_I1. apply* binds_concat_left.
+
+  assert (v<>y). intros neq. subst. apply ok_push_inv in okg. destruct okg as [_ okg]. false binds_fresh_inv H1 okg.
+  apply ALen_Var_I2 with t. apply* binds_concat_left.
+
+  destruct (eq_var_dec v y). subst.
+  apply ALen_Var. apply* binds_push_eq.
+
+  apply ALen_Var_I. auto_star.
+
+  inversion len; subst. apply ALen_EVar.
+  assert (v<>y). intros neq. subst. apply ok_push_inv in okg. destruct okg as [_ okg]. false binds_fresh_inv H1 okg.
+  apply* binds_concat_left.
+
+  assert (v<>y). intros neq. subst. apply ok_push_inv in okg. destruct okg as [_ okg]. false binds_fresh_inv H1 okg.
+  apply ALen_EVar_I1. apply* binds_concat_left.
+
+  assert (v<>y). intros neq. subst. apply ok_push_inv in okg. destruct okg as [_ okg]. false binds_fresh_inv H1 okg.
+  apply ALen_EVar_I2 with t. apply* binds_concat_left.
+
+  assert (v<>y). intros neq. subst. apply ok_push_inv in okg. destruct okg as [_ okg]. false binds_fresh_inv H1 okg.
+  apply ALen_EVar_I3 with t e. apply* binds_concat_left.
+
+  assert (v<>y). intros neq. subst. apply ok_push_inv in okg. destruct okg as [_ okg]. false binds_fresh_inv H0 okg.
+  apply ALen_Solved_EVar with t. apply* binds_concat_left.
+  apply* IHm. Omega.omega.
+
+  destruct (eq_var_dec v y). subst.
+  apply ALen_EVar_I1. apply* binds_push_eq.
+
+  apply ALen_EVar_I. auto_star.
+
+  inversion len; subst. apply ALen_Star.
+
+  inversion len; subst. apply ALen_App.
+  apply* IHe1. Omega.omega.
+  apply* IHe2. Omega.omega.
+
+  inversion len; subst. apply ALen_Lam.
+  apply* IHe. Omega.omega.
+
+  inversion len; subst. apply ALen_Pi.
+  apply* IHe1. Omega.omega.
+  apply* IHe2. Omega.omega.
+
+  inversion len; subst. apply ALen_Let.
+  apply* IHe1. Omega.omega.
+  apply* IHe2. Omega.omega.
+
+  inversion len; subst. apply ALen_CastUp.
+  apply* IHe. Omega.omega.
+
+  inversion len; subst. apply ALen_CastDn.
+  apply* IHe. Omega.omega.
+
+  inversion len; subst. apply ALen_Ann.
+  apply* IHe1. Omega.omega.
+  apply* IHe2. Omega.omega.
+Qed.
+
+Lemma alen_add_var: forall G e i y,
+    ALen G e i ->
+    ok (G & y ~ AC_Var) ->
+    ALen (G & y ~ AC_Var) e i.
+Proof.
+  introv len okg. apply* alen_add_var'.
+Qed.
+
+Lemma alen_open: forall G e i y,
+    ALen G e i ->
+    ok G ->
+    binds y AC_Var G ->
+    ALen G (e @ y) i.
+Proof.
+  introv len okg bd. unfold AOpen.
+  gen i. generalize 0. induction e; introv len; unfold AOpen; simpls; try(solve[assumption]).
+
+  case_if*. inversion len; subst. apply* ALen_Var.
+
+  inversion len; subst. apply ALen_App.
+  apply* IHe1. apply* IHe2.
+
+  inversion len; subst. apply ALen_Lam.
+  apply* IHe.
+
+  inversion len; subst. apply ALen_Pi.
+  apply* IHe1. apply* IHe2.
+
+  inversion len; subst. apply ALen_Let.
+  apply* IHe1. apply* IHe2.
+
+  inversion len; subst. apply ALen_CastUp.
+  apply* IHe.
+
+  inversion len; subst. apply ALen_CastDn.
+  apply* IHe.
+
+  inversion len; subst. apply ALen_Ann.
+  apply* IHe1. apply* IHe2.
+Qed.
+
+Lemma alen_awterm_append: forall G H e n,
+    AWf (G & H) ->
+    AWTermA G e ->
+    ALen G e n ->
+    ALen (G & H) e n.
+Proof.
+  introv wf wt len.
+  induction len.
+  auto.
+  apply ALen_Var. apply* binds_concat_left_ok. apply* awf_is_ok.
+  apply ALen_TypVar with t. apply* binds_concat_left_ok. apply* awf_is_ok.
+  apply* ALen_LetVar. apply* binds_concat_left_ok. apply* awf_is_ok. apply* IHlen. destruct (split_bind_context H0) as (G1 & G2 & Hg). rewrite Hg in wf.
+  assert (AWTerm G1 e).
+  rewrite <- concat_assoc in wf. apply AWf_left in wf. apply* awterm_bnd.
+  rewrite Hg. rewrite <- concat_assoc. apply* awterm_is_awterma. apply* awterm_weaken_ctx.
+  rewrite concat_assoc. apply AWf_left in wf. apply* awf_is_ok.
+
+  apply* ALen_Var_I1. apply* binds_concat_left_ok. apply* awf_is_ok.
+  apply* ALen_Var_I2. apply* binds_concat_left_ok. apply* awf_is_ok.
+  inversion wt; subst; try(solve[false binds_fresh_inv H3 H0]).
+
+  apply* ALen_EVar. apply* binds_concat_left_ok. apply* awf_is_ok.
+  apply* ALen_EVar_I1. apply* binds_concat_left_ok. apply* awf_is_ok.
+  apply* ALen_EVar_I2. apply* binds_concat_left_ok. apply* awf_is_ok.
+  apply* ALen_EVar_I3. apply* binds_concat_left_ok. apply* awf_is_ok.
+
+  apply* ALen_Solved_EVar. apply* binds_concat_left_ok. apply* awf_is_ok. apply* IHlen. destruct (split_bind_context H0) as (G1 & G2 & Hg). rewrite Hg in wf.
+  assert (AWTerm G1 t).
+  rewrite <- concat_assoc in wf. apply AWf_left in wf. apply* awterm_solved_evar.
+  rewrite Hg. rewrite <- concat_assoc. apply* awterm_is_awterma. apply* awterm_weaken_ctx.
+  rewrite concat_assoc. apply AWf_left in wf. apply* awf_is_ok.
+
+  inversion wt; subst; try(solve[false binds_fresh_inv H3 H0]).
+
+  apply* ALen_Star.
+  inversion wt; subst.
+  apply* ALen_App.
+  inversion wt; subst. apply* ALen_Lam.
+  inversion wt; subst. apply* ALen_Pi.
+  inversion wt; subst. apply* ALen_Let.
+  inversion wt; subst. apply* ALen_CastUp.
+  inversion wt; subst. apply* ALen_CastDn.
+  inversion wt; subst. apply* ALen_Ann.
+Qed.
+
+
+Lemma alen_exists': forall n G e,
+    AWf G ->
+    LibList.length G < n ->
+    exists m, ALen G e m.
+Proof.
+  intro n. induction n as [|n']; introv okg len.
+  false. inversion len.
+
+    induction e.
+  exists* 1.
+  assert ({v \in dom G}+{v \notin dom G}). apply* decidable_sumbool. apply indom_decidable.
+  destruct H as [hin | hnotin].
+  (* in *)
+  assert (exists vx, binds v vx G) by apply* get_some.
+  destruct H as (vx & H). destruct vx; auto_star.
+  destruct (split_bind_context H) as (G1 & G2 & IG).
+  assert (exists n, ALen G1 a0 n). apply~ IHn'.
+
+    rewrite IG in okg. rewrite <- concat_assoc in okg. apply* AWf_left.
+
+  rewrite IG in len.
+  rewrite concat_def in len. repeat(rewrite LibList.length_app in len).
+    assert(LibList.length (v~ AC_Bnd a a0) = 1). rewrite single_def. rewrite LibList.length_cons. rewrite LibList.length_nil. Omega.omega.
+
+  Omega.omega.
+
+    destruct H0 as (n & H0). exists* (n + 1). apply ALen_LetVar with a a0; auto.
+
+  rewrite <- concat_assoc in IG. rewrite IG. apply* alen_awterm_append. rewrite* <- IG. apply awterm_is_awterma. rewrite IG in okg. rewrite concat_assoc in okg. apply AWf_left in okg. apply* awterm_bnd.
+
+  (* notin *)
+
+  exists* 1.
+
+  assert ({v \in dom G}+{v \notin dom G}). apply* decidable_sumbool. apply indom_decidable.
+  destruct H as [hin | hnotin].
+  (* in *)
+  assert (exists vx, binds v vx G) by apply* get_some.
+  destruct H as (vx & H). destruct vx; auto_star.
+
+  destruct (split_bind_context H) as (G1 & G2 & IG).
+  assert (exists n, ALen G1 a n). apply~ IHn'.
+  rewrite IG in okg. rewrite <- concat_assoc in okg. apply* AWf_left.
+
+  rewrite IG in len.
+  rewrite concat_def in len. repeat(rewrite LibList.length_app in len).
+  assert(LibList.length (v~ AC_Solved_EVar a) = 1). rewrite single_def. rewrite LibList.length_cons. rewrite LibList.length_nil. Omega.omega.
+  Omega.omega.
+  destruct H0 as (ne & H0). exists (ne + 1). apply ALen_Solved_EVar with a; auto.
+  rewrite <- concat_assoc in IG. rewrite IG. apply* alen_awterm_append. rewrite* <- IG. apply awterm_is_awterma. rewrite IG in okg. rewrite concat_assoc in okg. apply AWf_left in okg. apply* awterm_solved_evar.
+
+  (* notin *)
+  exists* 1.
+
+  exists* 1.
+  destruct IHe1 as (n1 & IHe1). destruct IHe2 as (n2 & IHe2). exists* (n1 + n2 + 1).
+  destruct IHe as (n & IHe1). exists* (n + 1).
+  destruct IHe1 as (n1 & IHe1). destruct IHe2 as (n2 & IHe2). exists* (n1 + n2 + 1).
+  destruct IHe1 as (n1 & IHe1). destruct IHe2 as (n2 & IHe2). exists* (n1 + n2 + 1).
+  destruct IHe as (n & IHe1). exists* (n + 1).
+  destruct IHe as (n & IHe1). exists* (n + 1).
+  destruct IHe1 as (n1 & IHe1). destruct IHe2 as (n2 & IHe2). exists* (n1 + n2 + 1).
+Qed.
+
+Lemma alen_exists: forall G e,
+    AWf G ->
+    exists n, ALen G e n.
+Proof.
+  introv wf.
+  apply* alen_exists'.
+Qed.
+
+Lemma alen_eq: forall G e i1 i2,
+    ALen G e i1 ->
+    ALen G e i2 ->
+    i1 = i2.
+Proof.
+  introv hy1. gen i2. induction hy1; introv hy2; inversion hy2; subst; auto;
+  try(solve[apply (binds_func H) in H1; inversion H1]);
+  try(solve[apply (binds_func H) in H2; inversion H2]).
+  lets: binds_func H H1. inversion H0; subst. lets: IHhy1 i0 H3. subst*.
+  false binds_fresh_inv H H2.
+  false binds_fresh_inv H1 H.
+  lets: binds_func H H1. inversion H0; subst. lets: IHhy1 i0 H3. subst*.
+  false binds_fresh_inv H H2.
+  false binds_fresh_inv H1 H.
+Qed.
+
+Lemma alen_evar: forall G a t m n,
+    AWf G ->
+    binds a (AC_Solved_EVar t) G ->
+    ALen G (AE_EVar a) n ->
+    ALen G t m ->
+    n = m + 1.
+Proof.
+  introv wf bd lenn lenm.
+  inversion lenn; subst.
+  apply (binds_func H1) in bd; inversion bd.
+  apply (binds_func H1) in bd; inversion bd.
+  apply (binds_func H1) in bd; inversion bd.
+  apply (binds_func H1) in bd; inversion bd.
+  apply (binds_func bd) in H0; inversion H0; subst.
+  lets: alen_eq H2 lenm. subst*.
+  false binds_fresh_inv bd H1.
+Qed.
+
+Theorem cpltctxsubst_exists': forall G e n m,
+    AWf G ->
+    AWTerm G e ->
+    n < m ->
+    ALen G e n ->
+    CompleteCtx G ->
+    exists t, ACpltCtxSubst G e t
+.
+Proof.
+  intros. gen G e n. induction m; introv wf comp wt less len.
+  inversion less.
+
+  gen n. induction wt; introv less len; simpls; auto_star.
+  false (complete_contains_unsolved comp H).
+
+  assert (exists e, ACpltCtxSubst G t e).
+     destruct(@alen_exists G t) as (nt & ex). auto.
+     apply IHm with nt; auto. apply* awterm_evar_binds.
+     lets: alen_evar wf H len ex. rewrite H0 in less. Omega.omega.
+
+  destruct H0 as (et & H0).
+  exists et. destruct (split_bind_context H) as (G1 & G2 & HG). rewrite HG.
+  apply ACpltCtxSubst_EVar.
+  rewrite HG in comp. rewrite <- concat_assoc in comp. apply* complete_part_left. rewrite concat_assoc. rewrite HG in wf. apply* awf_is_ok.
+  rewrite HG in comp. apply* complete_part_right. rewrite HG in wf. apply* awf_is_ok.
+
+  apply* cpltctxsubst_solved_weaken. rewrite HG in wf. rewrite <- concat_assoc in wf. exact wf.
+  rewrite HG in comp. rewrite <- concat_assoc in comp. exact comp.
+  apply* awterm_solved_evar. rewrite HG in wf. apply AWf_left in wf. exact wf. rewrite concat_assoc. rewrite HG in H0. assumption.
+
+  destruct(@alen_exists G e1) as (ne1 & ex1). auto. auto. assert (exists t1, ACpltCtxSubst G e1 t1). apply* IHm.
+  inversion len; subst. lets: alen_eq H2 ex1. Omega.omega.
+  destruct H as (t1 & Ht1).
+  destruct(@alen_exists G e2) as (ne2 & ex2). auto. auto.
+  assert (exists t2, ACpltCtxSubst G e2 t2). apply* IHm.
+  inversion len; subst. lets: alen_eq H4 ex2. Omega.omega.
+  destruct H as (t2 & Ht2).
+  exists* (DE_App t1 t2).
+
+  inversion len; subst.
+  pick_fresh y.
+  assert (IH1: y \notin L) by auto_star.
+  assert (IH2: AWf (G & y ~ AC_Var)) by apply* AWf_Var.
+  assert (IH3: CompleteCtx (G & y ~ AC_Var)). unfold CompleteCtx. intros z zv bd eqzv. subst. apply binds_push_inv in bd. destruct bd as [[_ neq] | [_ neq]]. false neq. false complete_contains_unsolved comp neq.
+  assert (IH4: ALen (G & y ~ AC_Var) (e @ y) i).
+    apply alen_add_var with (y:=y) in H3.
+    apply* alen_open. apply* awf_is_ok. apply* awf_is_ok.
+  assert (IH5: i < S m). Omega.omega.
+  lets: H0 IH1 IH2 IH3 IH5 IH4.
+  destruct H1 as (et & H1).
+  apply* lam_solve.
+
+  inversion len; subst.
+  assert (IT1:  exists t, ACpltCtxSubst G t1 t). apply IHwt with (n:=i1); auto. Omega.omega.
+  pick_fresh y.
+  assert (IH1: y \notin L) by auto_star.
+  assert (IH2: AWf (G & y ~ AC_Var)) by apply* AWf_Var.
+  assert (IH3: CompleteCtx (G & y ~ AC_Var)). unfold CompleteCtx. intros z zv bd eqzv. subst. apply binds_push_inv in bd. destruct bd as [[_ neq] | [_ neq]]. false neq. false complete_contains_unsolved comp neq.
+  assert (IH4: ALen (G & y ~ AC_Var) (t2 @ y) i2).
+    apply alen_add_var with (y:=y) in H6.
+    apply* alen_open. apply* awf_is_ok. apply* awf_is_ok.
+  assert (IH5: i2 < S m). Omega.omega.
+  lets: H0 IH1 IH2 IH3 IH5 IH4.
+  destruct IT1 as (et1 & IT1).
+  destruct H1 as (et2 & H1).
+  apply* pi_solve.
+
+  inversion len; subst.
+  assert (IT1:  exists t, ACpltCtxSubst G e1 t). apply IHwt with (n:=i1); auto. Omega.omega.
+  pick_fresh y.
+  assert (IH1: y \notin L) by auto_star.
+  assert (IH2: AWf (G & y ~ AC_Var)) by apply* AWf_Var.
+  assert (IH3: CompleteCtx (G & y ~ AC_Var)). apply* complete_add.
+  assert (IH4: ALen (G & y ~ AC_Var) (e2 @ y) i2).
+    apply alen_add_var with (y:=y) in H6.
+    apply* alen_open. apply* awf_is_ok. apply* awf_is_ok.
+  assert (IH5: i2 < S m). Omega.omega.
+  lets: H0 IH1 IH2 IH3 IH5 IH4.
+  destruct IT1 as (et1 & IT1).
+  destruct H1 as (et2 & H1).
+  apply* let_solve.
+
+  assert (exists t, ACpltCtxSubst G e t).
+    destruct(@alen_exists G e) as (ne & ex). auto. auto. apply IHm with ne; auto.
+  inversion len; subst. lets: alen_eq H1 ex. Omega.omega.
+  destruct H as (et & H).
+  exists* (DE_CastUp et).
+
+  assert (exists t, ACpltCtxSubst G e t).
+    destruct(@alen_exists G e) as (ne & ex). auto. auto. apply IHm with ne; auto.
+  inversion len; subst. lets: alen_eq H1 ex. Omega.omega.
+  destruct H as (et & H).
+  exists* (DE_CastDn et).
+
+  destruct(@alen_exists G e1) as (ne1 & ex1). auto. auto. assert (exists t1, ACpltCtxSubst G e1 t1). apply* IHm.
+  inversion len; subst. lets: alen_eq H2 ex1. Omega.omega.
+  destruct H as (t1 & Ht1).
+  destruct(@alen_exists G e2) as (ne2 & ex2). auto. auto.
+  assert (exists t2, ACpltCtxSubst G e2 t2). apply* IHm.
+  inversion len; subst. lets: alen_eq H4 ex2. Omega.omega.
+  destruct H as (t2 & Ht2).
+  exists* (DE_Ann t1 t2).
+Qed.
+
+Theorem cpltctxsubst_exists: cpltctxsubst_exists_def.
+Proof.
+  introv. intros. destruct(@alen_exists G e) as (n & ex). auto. auto.
+  apply* cpltctxsubst_exists'.
+Qed.
+
+Theorem cpltctxtsubst_exists: cpltctxtsubst_exists_def.
+Proof.
+  introv wf wt comp.
+  induction wt.
+
+  pick_fresh y.
+  assert (IH1: y \notin L) by auto_star.
+  assert (IH2: AWf (G & y ~ AC_Var)). apply* AWf_Var.
+  assert (IH3: CompleteCtx (G & y ~ AC_Var)). apply* complete_add.
+  lets: H0 IH1 IH2 IH3.
+  destruct H1 as (nt & H1).
+  apply* forall_solve.
+
+  lets: cpltctxsubst_exists wf H comp.
+  destruct H0 as (nt & H0).
+  exists* (DT_Expr nt).
+  apply* ACpltCtxTSubst_Expr.
+Qed.
